Prove fixed_rate_currency_exchange in the new setting

proofs/fixed_rate_currency_exchange.v
@@ -1,143 +1,259 @@
-Load helpers.
+Load metaproperties.
 
-Definition currency_exchange_desc :=
+(* Fixed rate currency exchange *)
+Definition frce_desc :=
   (And
-     (Give (Scale 23 (One USD)))
-     (Scale 20 (One EUR))
+     (Give (Scale 11 (One USD)))
+     (Scale 10 (One EUR))
   ).
 
 
-Definition exchange_ctr
-           (alice bob : Address)
-           (ctr_id dsc_id : Id) :=
-  finctr ctr_id
-         dsc_id
-         currency_exchange_desc
-         alice
-         bob
-         bob
-         1.
-
-Ltac exec_exchange H :=
-  match type of H with
-  | exec_ctr_in_state_with_owner (exchange_ctr _ _ _ _) _ _ = Some _ =>
-    unfold exchange_ctr, currency_exchange_desc, exec_ctr_in_state_with_owner in H; simpl in H; inversion H; clear H
-  end.
-
-
-Lemma exchange_alice_gets_paid_by_bob :
-  forall s1 alice bob ctr_id dsc_id result,
-    exec_ctr_in_state_with_owner
-      (exchange_ctr alice bob ctr_id dsc_id) s1 bob =
+Print Transaction.
+Print execute.
+Lemma frce_execute_I_to_O :
+  forall sc I O bal time gtw ctr_id dsc_id next_id ledger result,
+    execute frce_desc sc I O bal time gtw ctr_id dsc_id next_id ledger =
     Some result ->
-    exists tr, # tr ∈ (res_ledger result) | ctr_id | bob --> alice | 23 $ USD #.
-Proof.
-  intros. exec_exchange H. subst result0.
-  simpl. eexists.
-  split.
-  - right. left. trivial.
-  - repeat split; trivial.
-Qed.
-
-
-Lemma exchange_alice_gets_paid_by_bob_step :
-  forall s1 s2 alice bob ctr_id dsc_id,
-    In (exchange_ctr alice bob ctr_id dsc_id)  (m_contracts s1) ->
-    s1 → s2 ⊢ ctr_id ->
-    bob <> 0 ->
-    exists result tr,
-      # tr ∈ (res_ledger result) | ctr_id | bob --> alice | 23 $ USD #.
-Proof.
-  intros until 1.
-  step_intro.
-  assert (H' := H0); auto.
-  induction H0; intros; set (EX := (exchange_ctr alice bob ctr_id0 dsc_id0)).
-  - unfold append_new_ctr_to_state in H8. subst s2. contradict_hyp H3.
-  - same_ctr ctr EX s2.
-    same_owner owner (ctr_owner EX) ctr EX.
-    subst ctr EX. subst owner. simpl in H9.
-    exists (result balance' ctrs' next' ledger').
-    eapply exchange_alice_gets_paid_by_bob.
-    exact H9.
-  - same_ctr ctr EX s2. subst ctr EX.
-    unfold exchange_ctr, currency_exchange_desc, ctr_primitive in H6. inversion H6.
-  - same_ctr ctr EX s2. subst ctr EX.
-    unfold exchange_ctr, currency_exchange_desc, ctr_primitive in H6. inversion H6.
-  - subst s2. contradict_hyp H3.
-  - subst s2. simpl in H3. contradiction.
-Qed.
-
-
-Theorem exchange_alice_gets_paid_by_bob_steps :
-  forall s1 s2 alice bob ctr_id dsc_id,
-    In (exchange_ctr alice bob ctr_id dsc_id)  (m_contracts s1) ->
-    s1 ⇓ s2 ⊢ ctr_id ->
-    bob <> 0 ->
-    exists result tr,
-      # tr ∈ (res_ledger result) | ctr_id | bob --> alice | 23 $ USD #.
+    exists tr,
+      In tr (res_ledger result) /\
+      tr_ctr_id tr = ctr_id /\
+      tr_from tr = I /\
+      tr_to tr = O /\
+      tr_amount tr = sc * 10 /\
+      tr_timestamp tr = time.
 Proof.
   intros.
-  assert (H' := H); auto.
-  eapply exists_step_in_steps in H'; eauto.
-  destruct H' as [s [s' [H3' [H5' [H6' H7']]]]].
-  eapply exchange_alice_gets_paid_by_bob_step; eauto.
-Qed.
-
-
-Lemma exchange_bob_gets_paid_by_alice :
-  forall s1 alice bob ctr_id dsc_id result,
-    exec_ctr_in_state_with_owner
-      (exchange_ctr alice bob ctr_id dsc_id) s1 bob =
-    Some result ->
-    exists tr, # tr ∈ (res_ledger result) | ctr_id | alice --> bob | 20 $ EUR #.
-Proof.
-  intros. exec_exchange H. subst result0.
-  simpl. eexists.
+  unfold frce_desc in H. simpl in H.
+  inversion H. clear H.
+  eexists. simpl.
   split.
   - left. trivial.
-  - repeat split; trivial.
+  - repeat split; simpl; trivial.
 Qed.
 
 
-Lemma exchange_bob_gets_paid_by_alice_step :
-  forall s1 s2 alice bob ctr_id dsc_id,
-    In (exchange_ctr alice bob ctr_id dsc_id)  (m_contracts s1) ->
-    s1 → s2 ⊢ ctr_id ->
-    bob <> 0 ->
-    exists result tr,
-      # tr ∈ (res_ledger result) | ctr_id | alice --> bob | 20 $ EUR #.
-Proof.
-  intros until 1.
-  step_intro.
-  assert (H' := H0); auto.
-  induction H0; intros; set (EX := (exchange_ctr alice bob ctr_id0 dsc_id0)).
-  - unfold append_new_ctr_to_state in H8. subst s2. contradict_hyp H3.
-  - same_ctr ctr EX s2.
-    same_owner owner (ctr_owner EX) ctr EX.
-    subst ctr EX. subst owner. simpl in H9.
-    exists (result balance' ctrs' next' ledger').
-    eapply exchange_bob_gets_paid_by_alice.
-    exact H9.
-  - same_ctr ctr EX s2. subst ctr EX.
-    unfold exchange_ctr, currency_exchange_desc, ctr_primitive in H6. inversion H6.
-  - same_ctr ctr EX s2. subst ctr EX.
-    unfold exchange_ctr, currency_exchange_desc, ctr_primitive in H6. inversion H6.
-  - subst s2. contradict_hyp H3.
-  - subst s2. simpl in H3. contradiction.
-Qed.
-
-
-Theorem exchange_bob_gets_paid_by_alice_steps :
-  forall s1 s2 alice bob ctr_id dsc_id,
-    In (exchange_ctr alice bob ctr_id dsc_id)  (m_contracts s1) ->
-    s1 ⇓ s2 ⊢ ctr_id ->
-    bob <> 0 ->
-    exists result tr,
-      # tr ∈ (res_ledger result) | ctr_id | alice --> bob | 20 $ EUR #.
+Lemma frce_execute_O_to_I :
+  forall sc I O bal time gtw ctr_id dsc_id next_id ledger result,
+    execute frce_desc sc I O bal time gtw ctr_id dsc_id next_id ledger =
+    Some result ->
+    exists tr,
+      In tr (res_ledger result) /\
+      tr_ctr_id tr = ctr_id /\
+      tr_from tr = O /\
+      tr_to tr = I /\
+      tr_amount tr = sc * 11 /\
+      tr_timestamp tr = time.
 Proof.
   intros.
-  assert (H' := H); auto.
-  eapply exists_step_in_steps in H'; eauto.
-  destruct H' as [s [s' [H3' [H5' [H6' H7']]]]].
-  eapply exchange_bob_gets_paid_by_alice_step; eauto.
+  unfold frce_desc in H. simpl in H.
+  inversion H. clear H.
+  eexists. simpl.
+  split.
+  - right. left. trivial.
+  - repeat split; simpl; trivial.
+Qed.
+
+Lemma frce_step_I_to_O:
+  forall s1 s2 ctr ctr_id dsc_id I O sc,
+    step s1 s2 ->
+    consistent_state s1 ->
+    ctr = finctr ctr_id dsc_id frce_desc I O O sc ->
+    In ctr (m_contracts s1) ->
+    ~ In (Executed ctr_id) (m_events s1) ->
+    In (Executed ctr_id) (m_events s2) ->
+    O <> 0 ->
+    exists tr,
+      In tr (m_ledger s2) /\
+      tr_ctr_id tr = ctr_id /\
+      tr_from tr = I /\
+      tr_to tr = O /\
+      tr_amount tr = sc * 10 /\
+      tr_timestamp tr = (m_global_time s1).
+Proof.
+  intros *.
+  intros H.
+  assert (H' := H).
+  induction H; intros.
+  - subst s2; simpl in *. destruct H9 as [H9 | H9]; try inversion H9; try contradiction.
+  - apply step_executes_only_one_contract with
+        (ctr := ctr) (ctr' := ctr0) in H'; auto.
+    + subst s2. simpl.
+      unfold can_join in H0.
+      destruct H0 as [H0 | H0]; try contradiction.
+      * subst owner ctr0.
+        rewrite H8 in H5.
+        unfold exec_ctr_in_state_with_owner in H5.
+        simpl in H5.
+        inversion H5.
+        eexists. simpl.
+        split.
+        ** left. trivial.
+        ** repeat split; trivial.
+      * subst ctr0 ctr. simpl in H0. rewrite H0 in H12. contradiction.
+    + subst ctr. simpl. trivial.
+    + subst s2. simpl. left. trivial.
+  - apply step_executes_only_one_contract with
+        (ctr := ctr) (ctr' := ctr0) in H'; auto.
+    + subst ctr ctr0. unfold frce_desc in H2. simpl in H2. inversion H2.
+    + subst ctr. simpl. trivial.
+    + subst s2. simpl. left. trivial.
+  - apply step_executes_only_one_contract with
+        (ctr := ctr) (ctr' := ctr0) in H'; auto.
+    + subst ctr ctr0. unfold frce_desc in H2. simpl in H2. inversion H2.
+    + subst ctr. simpl. trivial.
+    + subst s2. simpl. left. trivial.
+  - subst s2. simpl in *.
+    destruct H9 as [H9 | H9]; try contradiction; try inversion H9.
+  - subst s2. simpl in *. contradiction.
+Qed.
+
+
+Lemma frce_step_O_to_I:
+  forall s1 s2 ctr ctr_id dsc_id I O sc,
+    step s1 s2 ->
+    consistent_state s1 ->
+    ctr = finctr ctr_id dsc_id frce_desc I O O sc ->
+    In ctr (m_contracts s1) ->
+    ~ In (Executed ctr_id) (m_events s1) ->
+    In (Executed ctr_id) (m_events s2) ->
+    O <> 0 ->
+    exists tr,
+      In tr (m_ledger s2) /\
+      tr_ctr_id tr = ctr_id /\
+      tr_from tr = O /\
+      tr_to tr = I /\
+      tr_amount tr = sc * 11 /\
+      tr_timestamp tr = (m_global_time s1).
+Proof.
+  intros *.
+  intros H.
+  assert (H' := H).
+  induction H; intros.
+  - subst s2; simpl in *. destruct H9 as [H9 | H9]; try inversion H9; try contradiction.
+  - apply step_executes_only_one_contract with
+        (ctr := ctr) (ctr' := ctr0) in H'; auto.
+    + subst s2. simpl.
+      unfold can_join in H0.
+      destruct H0 as [H0 | H0]; try contradiction.
+      * subst owner ctr0.
+        rewrite H8 in H5.
+        unfold exec_ctr_in_state_with_owner in H5.
+        simpl in H5.
+        inversion H5.
+        eexists. simpl.
+        split.
+        ** right. left. trivial.
+        ** repeat split; trivial.
+      * subst ctr0 ctr. simpl in H0. rewrite H0 in H12. contradiction.
+    + subst ctr. simpl. trivial.
+    + subst s2. simpl. left. trivial.
+  - apply step_executes_only_one_contract with
+        (ctr := ctr) (ctr' := ctr0) in H'; auto.
+    + subst ctr ctr0. unfold frce_desc in H2. simpl in H2. inversion H2.
+    + subst ctr. simpl. trivial.
+    + subst s2. simpl. left. trivial.
+  - apply step_executes_only_one_contract with
+        (ctr := ctr) (ctr' := ctr0) in H'; auto.
+    + subst ctr ctr0. unfold frce_desc in H2. simpl in H2. inversion H2.
+    + subst ctr. simpl. trivial.
+    + subst s2. simpl. left. trivial.
+  - subst s2. simpl in *.
+    destruct H9 as [H9 | H9]; try contradiction; try inversion H9.
+  - subst s2. simpl in *. contradiction.
+Qed.
+
+
+Lemma frce_steps_I_to_O:
+  forall s1 s2 ctr ctr_id dsc_id I O sc,
+    steps s1 s2 ->
+    consistent_state s1 ->
+    ctr = finctr ctr_id dsc_id frce_desc I O O sc ->
+    In ctr (m_contracts s1) ->
+    ~ In (Executed ctr_id) (m_events s1) ->
+    In (Executed ctr_id) (m_events s2) ->
+    O <> 0 ->
+    exists time tr,
+      In tr (m_ledger s2) /\
+      tr_ctr_id tr = ctr_id /\
+      tr_from tr = I /\
+      tr_to tr = O /\
+      tr_amount tr = sc * 10 /\
+      tr_timestamp tr = time.
+Proof.
+  intros.
+  induction H; intros.
+  - subst. contradiction.
+  - assert (H' := H).
+    apply steps_preserves_consistent_state in H'; auto.
+    apply steps_effect_over_contract with (ctr := ctr) in H; trivial.
+    destruct H as [H|[H|H]]; trivial.
+    + eexists.
+      eapply frce_step_I_to_O; eauto.
+      destruct H' as [H' [T P]].
+      apply T in H.
+      destruct H as [H _].
+      subst ctr.
+      simpl in *.
+      trivial.
+    + subst ctr.
+      simpl in *.
+      apply IHsteps in H.
+      destruct H as [time [tr [S2 H]]].
+      exists time, tr.
+      split; trivial.
+      eapply step_does_not_remove_transactions; eauto.
+    + eapply step_does_not_remove_events in H; eauto.
+      eapply step_preserves_consistent_state in H'; eauto.
+      destruct H' as [H' [T P]].
+      subst ctr. simpl in *.
+      contradiction P with (e := ctr_id0).
+      split; trivial.
+Qed.
+
+
+Lemma frce_steps_O_to_I:
+  forall s1 s2 ctr ctr_id dsc_id O I sc,
+    steps s1 s2 ->
+    consistent_state s1 ->
+    ctr = finctr ctr_id dsc_id frce_desc I O O sc ->
+    In ctr (m_contracts s1) ->
+    ~ In (Executed ctr_id) (m_events s1) ->
+    In (Executed ctr_id) (m_events s2) ->
+    O <> 0 ->
+    exists time tr,
+      In tr (m_ledger s2) /\
+      tr_ctr_id tr = ctr_id /\
+      tr_from tr = O /\
+      tr_to tr = I /\
+      tr_amount tr = sc * 11 /\
+      tr_timestamp tr = time.
+Proof.
+  intros.
+  induction H; intros.
+  - subst. contradiction.
+  - assert (H' := H).
+    apply steps_preserves_consistent_state in H'; auto.
+    apply steps_effect_over_contract with (ctr := ctr) in H; trivial.
+    destruct H as [H|[H|H]]; trivial.
+    + eexists.
+      eapply frce_step_O_to_I; eauto.
+      destruct H' as [H' [T P]].
+      apply T in H.
+      destruct H as [H _].
+      subst ctr.
+      simpl in *.
+      trivial.
+    + subst ctr.
+      simpl in *.
+      apply IHsteps in H.
+      destruct H as [time [tr [S2 H]]].
+      exists time, tr.
+      split; trivial.
+      eapply step_does_not_remove_transactions; eauto.
+    + eapply step_does_not_remove_events in H; eauto.
+      eapply step_preserves_consistent_state in H'; eauto.
+      destruct H' as [H' [T P]].
+      subst ctr. simpl in *.
+      contradiction P with (e := ctr_id0).
+      split; trivial.
 Qed.
